cellio/MainHeader.v
@@ -1,6 +1,0 @@
-Require Import CRIS.
-
-Module MainHdr.
-  Definition main : option string := None.
-
-End MainHdr.
